concurrency/Clight_bounds.v
@@ -1,0 +1,48 @@
+Require Import compcert.lib.Axioms.
+Require Import compcert.lib.Maps.
+
+Require Import concurrency.sepcomp. Import SepComp.
+
+Require Import concurrency.pos.
+Require Import concurrency.scheduler.
+Require Import concurrency.TheSchedule.
+Require Import concurrency.konig.
+Require Import concurrency.addressFiniteMap. (*The finite maps*)
+Require Import concurrency.pos.
+Require Import concurrency.lksize.
+Require Import concurrency.permjoin_def.
+Require Import Coq.Program.Program.
+From mathcomp.ssreflect Require Import ssreflect ssrbool ssrnat ssrfun eqtype seq fintype finfun.
+Set Implicit Arguments.
+
+
+Require Import Coq.ZArith.ZArith.
+
+Require Import concurrency.permissions.
+Require Import concurrency.threadPool.
+ 
+Require Import compcert.common.Memory. (*for Mem.perm_order'' *)
+Require Import concurrency.bounded_maps.
+
+
+(*Semantics*)
+Require Import veric.Clight_new.
+Require Import veric.Clightnew_coop.
+Require Import sepcomp.event_semantics.
+Require Import veric.Clight_sim.
+Require Import concurrency.ClightSemantincsForMachines.
+
+
+Lemma CLight_Deterministic: forall ge c m c1 m1 c2 m2,
+    veric.Clight_new.cl_step ge c m c2 m2 ->
+    veric.Clight_new.cl_step ge c m c1 m1 ->
+    c1 = c2 /\ m1 = m2.
+                
+Admitted.
+
+Lemma CLight_step_mem_bound: forall ge c m c' m',
+    veric.Clight_new.cl_step ge c m c' m' ->
+    bounded_maps.bounded_map (snd (getMaxPerm m)) ->
+    bounded_maps.bounded_map (snd (getMaxPerm m')).
+                
+Admitted.
